src/DRandom.dfy
@@ -6,21 +6,27 @@
 // RUN: %verify "%s"
 
 include "Distributions/Base/Interface.dfy"
-include "Distributions/Bernoulli/Interface.dfy"
-include "Distributions/BernoulliExp/Interface.dfy"
-include "Distributions/DiscreteGaussian/Interface.dfy"
-include "Distributions/DiscreteLaplace/Interface.dfy"
-include "Distributions/Geometric/Interface.dfy"
-include "Distributions/Uniform/Interface.dfy"
+include "Distributions/Bernoulli/Implementation.dfy"
+include "Distributions/BernoulliExpNeg/Implementation.dfy"
+include "Distributions/DiscreteGaussian/Implementation.dfy"
+include "Distributions/DiscreteLaplace/Implementation.dfy"
+include "Distributions/Geometric/Implementation.dfy"
+include "Distributions/Uniform/Implementation.dfy"
 
 module {:extern "DafnyLibraries"} DafnyLibraries {
+  import opened Base
+  import opened Bernoulli
+  import opened Geometric
+  import opened Uniform
+  import opened BernoulliExpNeg
+  import opened DiscreteGaussian
+  import opened DiscreteLaplace
 
-  class {:extern} DRandomFoundational extends Base, Unif, Bernoulli__, UniformFoundational, BernoulliExpNeg, DiscreteGaussian, DiscreteLaplace {
+  class {:extern} DRandomFoundational extends Base, Unif, Bernoulli, Geometric, UniformFoundational, BernoulliExpNeg, DiscreteGaussian, DiscreteLaplace {
     constructor {:extern} ()
   }
 
-  class {:extern} DRandomExternUniform extends Base, Unif, Bernoulli__, UniformExtern, BernoulliExpNeg, DiscreteGaussian, DiscreteLaplace {
+  class {:extern} DRandomExternUniform extends Base, Unif, Bernoulli, Geometric, UniformExtern, BernoulliExpNeg, DiscreteGaussian, DiscreteLaplace {
     constructor {:extern} ()
   }
-
 }
