src/Distributions/Bernoulli/Implementation.dfy
@@ -7,39 +7,22 @@ include "../../Math/MeasureTheory.dfy"
 include "Interface.dfy"
 include "Model.dfy"
 
-import opened MeasureTheory
-import opened BernoulliModel
+module Bernoulli {
+  import opened MeasureTheory
+  import opened BernoulliModel
+  import opened IBernoulli
 
-trait Bernoulli__ extends IBernoulli {
+  trait {:termination false} Bernoulli extends IBernoulli {
 
-  method Bernoulli(p: real) returns (c: bool)
-    modifies this
-    decreases *
-    requires 0.0 <= p <= 1.0
-    ensures ProbBernoulli(p)(old(s)) == (c, s)
-  {
-    var q: Probability := p as real;
-
-    var b := Coin();
-    if b {
-      if q <= 0.5 {
-        return false;
-      } else {
-        q := 2.0 * (q as real) - 1.0;
-      }
-    } else {
-      if q <= 0.5 {
-        q := 2.0 * (q as real);
-      } else {
-        return true;
-      }
-    }
-
-    while true
-      invariant ProbBernoulli(p)(old(s)) == ProbBernoulli(q)(s)
+    method Bernoulli(p: real) returns (c: bool)
+      modifies this
       decreases *
+      requires 0.0 <= p <= 1.0
+      ensures ProbBernoulli(p)(old(s)) == (c, s)
     {
-      b := Coin();
+      var q: Probability := p as real;
+
+      var b := Coin();
       if b {
         if q <= 0.5 {
           return false;
@@ -53,7 +36,27 @@ trait Bernoulli__ extends IBernoulli {
           return true;
         }
       }
-    }
-  }
 
+      while true
+        invariant ProbBernoulli(p)(old(s)) == ProbBernoulli(q)(s)
+        decreases *
+      {
+        b := Coin();
+        if b {
+          if q <= 0.5 {
+            return false;
+          } else {
+            q := 2.0 * (q as real) - 1.0;
+          }
+        } else {
+          if q <= 0.5 {
+            q := 2.0 * (q as real);
+          } else {
+            return true;
+          }
+        }
+      }
+    }
+
+  }
 }
