src/Distributions/BernoulliExpNeg/Implementation.dfy
@@ -6,35 +6,40 @@
 include "../Bernoulli/Interface.dfy"
 include "Interface.dfy"
 
-trait BernoulliExpNeg extends IBernoulli, IBernoulliExpNeg {
+module BernoulliExpNeg {
+  import opened IBernoulli
+  import opened IBernoulliExpNeg
 
-  // Based on Algorithm 1 in https://arxiv.org/pdf/2004.00010.pdf; unverified
-  method BernoulliExpNeg(gamma: real) returns (c: bool)
-    modifies this
-    decreases *
-    requires gamma >= 0.0
-  {
-    if gamma <= 1.0 {
-      var k := 1;
-      var a := Bernoulli(gamma / (k as real));
-      while a
-        decreases *
-      {
-        k := k + 1;
-        a := Bernoulli(gamma / (k as real));
-      }
-      c := k % 2 == 1;
-    } else {
-      var k := 1;
-      while k <= gamma.Floor {
-        var b := BernoulliExpNeg(1.0);
-        if !b {
-          return false;
+  trait {:termination false} BernoulliExpNeg extends IBernoulli, IBernoulliExpNeg {
+
+    // Based on Algorithm 1 in https://arxiv.org/pdf/2004.00010.pdf; unverified
+    method BernoulliExpNeg(gamma: real) returns (c: bool)
+      modifies this
+      decreases *
+      requires gamma >= 0.0
+    {
+      if gamma <= 1.0 {
+        var k := 1;
+        var a := Bernoulli(gamma / (k as real));
+        while a
+          decreases *
+        {
+          k := k + 1;
+          a := Bernoulli(gamma / (k as real));
         }
-        k := k + 1;
+        c := k % 2 == 1;
+      } else {
+        var k := 1;
+        while k <= gamma.Floor {
+          var b := BernoulliExpNeg(1.0);
+          if !b {
+            return false;
+          }
+          k := k + 1;
+        }
+        c:= BernoulliExpNeg(gamma - gamma.Floor as real);
       }
-      c:= BernoulliExpNeg(gamma - gamma.Floor as real);
     }
-  }
 
+  }
 }
