src/Distributions/DiscreteGaussian/Interface.dfy
@@ -6,13 +6,14 @@
 include "../BernoulliExpNeg/Interface.dfy"
 include "../DiscreteLaplace/Interface.dfy"
 
-trait IDiscreteGaussian extends IDiscreteLaplace, IBernoulliExpNeg {
+module IDiscreteGaussian {
+  import opened IBernoulliExpNeg
+  import opened IDiscreteLaplace
 
-  // Based on Algorithm 3 in https://arxiv.org/pdf/2004.00010.pdf; unverified
-  // Note that we take sigma as a parameter, not sigma^2, to avoid square roots.
-  method DiscreteGaussian(sigma: real) returns (y: int)
-    modifies this
-    requires sigma > 0.0
-    decreases *
-
+  trait {:termination false} IDiscreteGaussian extends IDiscreteLaplace, IBernoulliExpNeg {
+    method DiscreteGaussian(sigma: real) returns (y: int)
+      modifies this
+      requires sigma > 0.0
+      decreases *
+  }
 }
