src/Distributions/DiscreteLaplace/Implementation.dfy
@@ -5,40 +5,44 @@
 
 include "Interface.dfy"
 
-trait DiscreteLaplace extends IDiscreteLaplace {
+module DiscreteLaplace {
+  import opened IDiscreteLaplace
 
-  // Based on Algorithm 2 in https://arxiv.org/pdf/2004.00010.pdf; unverified
-  method DiscreteLaplace(s: nat, t: nat) returns (z: int)
-    modifies this
-    requires s >= 1
-    requires t >= 1
-    decreases *
-  {
-    var b := true;
-    var y := 0;
-    while b && y == 0
+  trait {:termination false} DiscreteLaplace extends IDiscreteLaplace {
+
+    // Based on Algorithm 2 in https://arxiv.org/pdf/2004.00010.pdf; unverified
+    method DiscreteLaplace(s: nat, t: nat) returns (z: int)
+      modifies this
+      requires s >= 1
+      requires t >= 1
       decreases *
     {
-      var u := Uniform(t);
-      var d := BernoulliExpNeg(u as real / t as real);
-      if !d {
-        continue;
-      }
-      var v := 0;
-      var a := true;
-      while a
+      var b := true;
+      var y := 0;
+      while b && y == 0
         decreases *
       {
-        a := BernoulliExpNeg(1.0);
-        if a {
-          v := v + 1;
+        var u := Uniform(t);
+        var d := BernoulliExpNeg(u as real / t as real);
+        if !d {
+          continue;
         }
+        var v := 0;
+        var a := true;
+        while a
+          decreases *
+        {
+          a := BernoulliExpNeg(1.0);
+          if a {
+            v := v + 1;
+          }
+        }
+        var x := u + t * v;
+        y := x / s;
+        b := Bernoulli(0.5);
       }
-      var x := u + t * v;
-      y := x / s;
-      b := Bernoulli(0.5);
+      z := if b then -y else y;
     }
-    z := if b then -y else y;
-  }
 
+  }
 }
