src/Distributions/DiscreteLaplace/Interface.dfy
@@ -7,13 +7,19 @@ include "../Bernoulli/Interface.dfy"
 include "../Uniform/Interface.dfy"
 include "../BernoulliExpNeg/Interface.dfy"
 
-trait IDiscreteLaplace extends IBernoulli, IUniform, IBernoulliExpNeg {
+module IDiscreteLaplace {
+  import opened IBernoulli
+  import opened IUniform
+  import opened IBernoulliExpNeg
 
-  // Based on Algorithm 2 in https://arxiv.org/pdf/2004.00010.pdf; unverified
-  method DiscreteLaplace(s: nat, t: nat) returns (z: int)
-    modifies this
-    requires s >= 1
-    requires t >= 1
-    decreases *
+  trait {:termination false} IDiscreteLaplace extends IBernoulli, IUniform, IBernoulliExpNeg {
 
+    // Based on Algorithm 2 in https://arxiv.org/pdf/2004.00010.pdf; unverified
+    method DiscreteLaplace(s: nat, t: nat) returns (z: int)
+      modifies this
+      requires s >= 1
+      requires t >= 1
+      decreases *
+
+  }
 }
