src/Distributions/Geometric/Interface.dfy
@@ -6,13 +6,18 @@
 include "../../ProbabilisticProgramming/Monad.dfy"
 include "../Base/Interface.dfy"
 
-trait IGeometric extends Base {
+module IGeometric {
+  import opened Base
+  import opened Monad
 
-  method Geometric() returns (c: nat)
-    modifies this
-    decreases *
-    ensures !old(s)(c)
-    ensures forall i | 0 <= i < c :: old(s)(i)
-    ensures s == Monad.IterateTail(old(s), c + 1)
+  trait {:termination false} IGeometric extends Base {
 
+    method Geometric() returns (c: nat)
+      modifies this
+      decreases *
+      ensures !old(s)(c)
+      ensures forall i | 0 <= i < c :: old(s)(i)
+      ensures s == Monad.IterateTail(old(s), c + 1)
+
+  }
 }
