src/Distributions/Uniform/Interface.dfy
@@ -6,21 +6,39 @@
 include "../Base/Interface.dfy"
 include "Model.dfy"
 
-trait IUniform extends Base, IUnif {
+module IUniform {
+  import opened Base
+  import opened UniformModel
 
-  method Uniform(n: nat) returns (u: nat)
-    modifies this
-    decreases *
-    requires n > 0
-    ensures u < n
-    ensures UniformModel.ProbUniform(n)(old(s)) == (u, s)
+  trait {:termination false} IUniform extends Base, IUnif {
 
-}
+    method Uniform(n: nat) returns (u: nat)
+      modifies this
+      decreases *
+      requires n > 0
+      ensures u < n
+      ensures UniformModel.ProbUniform(n)(old(s)) == (u, s)
 
-trait IUnif extends Base {
+      method UniformInterval(a: int, b: int) returns (u: int)
+        modifies this
+        decreases *
+        requires a < b
+        ensures a <= u < b
+        ensures UniformModel.ProbUniformInterval(a, b)(old(s)) == (u, s)
+      {
+        var v := Uniform(b - a);
+        assert UniformModel.ProbUniform(b-a)(old(s)) == (v, s);
+        assert UniformModel.ProbUniformInterval(a, b)(old(s)) == (a + v, s);
+        u := a + v;
+      }
 
-  method Unif(n: nat) returns (u: nat)
-    modifies this
-    ensures UniformModel.ProbUnif(n)(old(s)) == (u, s)
+  }
 
+  trait {:termination false} IUnif extends Base {
+
+    method Unif(n: nat) returns (u: nat)
+      modifies this
+      ensures UniformModel.ProbUnif(n)(old(s)) == (u, s)
+
+  }
 }
